{
 "cells": [
  {
   "cell_type": "markdown",
   "id": "fd7315de",
   "metadata": {},
   "source": [
    "$\\textbf{Question 10  :}$\n",
    "\n",
    "Given the matrix $ ùê¥ = \\begin{bmatrix} 2 & 1 \\\\ 1 & 2 \\end{bmatrix} $, answer the following questions, by providing all the necessary\n",
    "by-hand calculations:\n",
    "(i) Compute the characteristic polynomial and the eigenvalues of the matrix ùê¥.\n",
    "(ii) Compute the eigenvectors of the matrix ùê¥.\n",
    "(iii) Find a general formula for the matrix ùê¥ùëõ with ùëõ ‚àà ‚Ñ§+, utilizing the diagonalizable nature\n",
    "of the original matrix ùê¥.\n",
    "\n",
    "$\\textbf{Answer :}$"
   ]
  },
  {
   "cell_type": "markdown",
   "id": "b48d4414",
   "metadata": {},
   "source": [
    "To find the characteristic polynomial and eigenvalues of matrix $A = \\begin{bmatrix} 2 & 1 \\\\ 1 & 2 \\end{bmatrix}$, we need to solve the characteristic equation, which is given by:\n",
    "\n",
    "$ \\text{det}(A - \\lambda I) = 0 $\n",
    "\n",
    "where $ \\lambda $ is the eigenvalue, $I$ is the identity matrix, and $\\text{det}$ denotes the determinant.\n",
    "\n",
    "Let $A - \\lambda I$ be the matrix:\n",
    "\n",
    "$ A - \\lambda I = \\begin{bmatrix} 2 - \\lambda & 1 \\\\ 1 & 2 - \\lambda \\end{bmatrix} $\n",
    "\n",
    "Now, find the determinant of this matrix and set it equal to zero:\n",
    "\n",
    "$ \\text{det}(A - \\lambda I) = (2 - \\lambda)(2 - \\lambda) - (1)(1) = (2 - \\lambda)^2 - 1 $\n",
    "\n",
    "Now, set the determinant equal to zero:\n",
    "\n",
    "$ (2 - \\lambda)^2 - 1 = 0 $\n",
    "\n",
    "Expand and solve for $\\lambda$:\n",
    "\n",
    "$ (2 - \\lambda)^2 = 1 $\n",
    "\n",
    "Taking the square root of both sides:\n",
    "\n",
    "$ 2 - \\lambda = \\pm 1 $\n",
    "\n",
    "Solving for $\\lambda$, we get two possible eigenvalues:\n",
    "\n",
    "1. When $2 - \\lambda = 1 $:\n",
    "   $ \\lambda_1 = 2 - 1 = 1 $\n",
    "\n",
    "2. When $2 - \\lambda = -1 $:\n",
    "   $ \\lambda_2 = 2 + 1 = 3 $\n",
    "\n",
    "So, the eigenvalues of matrix $A$ are $\\lambda_1 = 1$ and $\\lambda_2 = 3$.\n",
    "\n",
    "The characteristic polynomial is given by the expression obtained when we set $\\text{det}(A - \\lambda I)$ equal to zero:\n",
    "\n",
    "$ \\text{char}(A) = (2 - \\lambda)^2 - 1 $"
   ]
  },
  {
   "cell_type": "markdown",
   "id": "eafbebaa",
   "metadata": {},
   "source": [
    "\n",
    "(ii) Compute the eigenvectors of the matrix ùê¥.\n",
    "\n",
    "$\\textbf{Answer :}$"
   ]
  },
  {
   "cell_type": "markdown",
   "id": "f814dd17",
   "metadata": {},
   "source": [
    "To compute the eigenvectors corresponding to each eigenvalue, we need to solve the system of linear equations $(A - \\lambda I) \\mathbf{v} = \\mathbf{0}$, where $\\lambda$ is each eigenvalue and $\\mathbf{v}$ is the corresponding eigenvector.\n",
    "\n",
    "For $\\lambda_1 = 1$:\n",
    "\n",
    "$ (A - \\lambda_1 I) \\mathbf{v}_1 = \\begin{bmatrix} 1 & 1 \\\\ 1 & 1 \\end{bmatrix} \\begin{bmatrix} x \\\\ y \\end{bmatrix} = \\begin{bmatrix} 0 \\\\ 0 \\end{bmatrix} $\n",
    "\n",
    "This system of equations can be expressed as:\n",
    "\n",
    "$ x + y = 0 $\n",
    "\n",
    "This implies that $y = -x$. Letting $x = 1$, we get the eigenvector $\\mathbf{v}_1 = \\begin{bmatrix} 1 \\\\ -1 \\end{bmatrix}$.\n",
    "\n",
    "For $\\lambda_2 = 3$:\n",
    "\n",
    "$ (A - \\lambda_2 I) \\mathbf{v}_2 = \\begin{bmatrix} -1 & 1 \\\\ 1 & -1 \\end{bmatrix} \\begin{bmatrix} x \\\\ y \\end{bmatrix} = \\begin{bmatrix} 0 \\\\ 0 \\end{bmatrix} $\n",
    "\n",
    "This system of equations can be expressed as:\n",
    "\n",
    "$ -x + y = 0 $\n",
    "\n",
    "This implies that $y = x$. Letting $x = 1$, we get the eigenvector $\\mathbf{v}_2 = \\begin{bmatrix} 1 \\\\ 1 \\end{bmatrix}$.\n",
    "\n",
    "So, the eigenvectors corresponding to the eigenvalues $\\lambda_1 = 1$ and $\\lambda_2 = 3$ are $\\mathbf{v}_1 = \\begin{bmatrix} 1 \\\\ -1 \\end{bmatrix}$ and $\\mathbf{v}_2 = \\begin{bmatrix} 1 \\\\ 1 \\end{bmatrix}$, respectively."
   ]
  },
  {
   "cell_type": "markdown",
   "id": "b290de93",
   "metadata": {},
   "source": [
    "\n",
    "(iii) Find a general formula for the matrix ùê¥ùëõ with ùëõ ‚àà ‚Ñ§+, utilizing the diagonalizable nature\n",
    "of the original matrix ùê¥.\n",
    "\n",
    "$\\textbf{Answer :}$"
   ]
  },
  {
   "cell_type": "markdown",
   "id": "6d6d3e7c",
   "metadata": {},
   "source": [
    "Since matrix $A$ is diagonalizable (having distinct eigenvalues), we can express it as $A = PDP^{-1}$, where $D$ is the diagonal matrix of eigenvalues and $P$ is the matrix whose columns are the corresponding eigenvectors.\n",
    "\n",
    "The general formula for $A^n$ can then be obtained by raising the diagonal matrix $D$ to the power of $n$:\n",
    "\n",
    "$ A^n = (PDP^{-1})^n = PD^nP^{-1} $\n",
    "\n",
    "where $D^n$ is obtained by raising each diagonal element of $D$ to the power of $n$.\n",
    "\n",
    "Since $D$ is a diagonal matrix with eigenvalues $\\lambda_1, \\lambda_2, \\ldots, \\lambda_k$, and $\\mathbf{v}_1, \\mathbf{v}_2, \\ldots, \\mathbf{v}_k$ are the corresponding eigenvectors forming the columns of $P$, the formula becomes:\n",
    "\n",
    "$ A^n = P \\begin{bmatrix} \\lambda_1^n & 0 & \\ldots & 0 \\\\ 0 & \\lambda_2^n & \\ldots & 0 \\\\ \\vdots & \\vdots & \\ddots & \\vdots \\\\ 0 & 0 & \\ldots & \\lambda_k^n \\end{bmatrix} P^{-1} $\n",
    "\n",
    "So, the general formula for $A^n$ is given by this expression involving the diagonalization of $A$.\n",
    "\n",
    "Since the matrix $A$ is diagonalizable with distinct eigenvalues $\\lambda_1 = 1$ and $\\lambda_2 = 3$, we can diagonalize $A$ as follows:\n",
    "\n",
    "$ A = PDP^{-1} $\n",
    "\n",
    "where $D$ is the diagonal matrix containing the eigenvalues of $A$ on the diagonal, and the columns of $P$ are the corresponding eigenvectors of $A$. Thus, we have:\n",
    "\n",
    "$ P = \\begin{bmatrix} 1 & 1 \\\\ -1 & 1 \\end{bmatrix} $\n",
    "$ D = \\begin{bmatrix} 1 & 0 \\\\ 0 & 3 \\end{bmatrix} $\n",
    "\n",
    "let's calculate the inverse of matrix $P$:\n",
    "\n",
    "$ P = \\begin{bmatrix} 1 & 1 \\\\ -1 & 1 \\end{bmatrix} $\n",
    "\n",
    "The inverse of a 2x2 matrix $\\begin{bmatrix} a & b \\\\ c & d \\end{bmatrix}$ is given by the formula:\n",
    "\n",
    "$ \\text{Inverse} = \\frac{1}{ad - bc} \\begin{bmatrix} d & -b \\\\ -c & a \\end{bmatrix} $\n",
    "\n",
    "So for matrix $P$, where $a = 1$, $b = 1$, $c = -1$, and $d = 1$, the inverse is:\n",
    "\n",
    "$ P^{-1} = \\frac{1}{(1)(1) - (1)(-1)} \\begin{bmatrix} 1 & -1 \\\\ 1 & 1 \\end{bmatrix} $\n",
    "\n",
    "$ P^{-1} = \\frac{1}{2} \\begin{bmatrix} 1 & -1 \\\\ 1 & 1 \\end{bmatrix} $\n",
    "\n",
    "Therefore, the inverse of matrix $P$ is:\n",
    "\n",
    "$ P^{-1} = \\frac{1}{2} \\begin{bmatrix} 1 & -1 \\\\ 1 & 1 \\end{bmatrix} $\n",
    "\n",
    "\n",
    "\n",
    "Now, let's compute $A^n$ for $n \\in \\mathbb{Z}^+$:\n",
    "\n",
    "$ A^n = (PDP^{-1})^n = PD^nP^{-1} $\n",
    "\n",
    "Where $D^n$ is the diagonal matrix with each diagonal entry raised to the $n$th power. For $D$, this is straightforward:\n",
    "\n",
    "$ D^n = \\begin{bmatrix} 1^n & 0 \\\\ 0 & 3^n \\end{bmatrix} = \\begin{bmatrix} 1 & 0 \\\\ 0 & 3^n \\end{bmatrix} $\n",
    "\n",
    "Now, we need to compute $P^{-1}P$, which equals the identity matrix $I$, so we have:\n",
    "\n",
    "$ PD^nP^{-1} = \\begin{bmatrix} 1 & 1 \\\\ -1 & 1 \\end{bmatrix} \\begin{bmatrix} 1 & 0 \\\\ 0 & 3^n \\end{bmatrix} \\frac{1}{2} \\begin{bmatrix} 1 & -1 \\\\ 1 & 1 \\end{bmatrix} $\n",
    "\n",
    "Let's compute this product:\n",
    "\n",
    "$ PD^nP^{-1} = \\frac{1}{2} \\begin{bmatrix} 1 & 1 \\\\ -1 & 1 \\end{bmatrix} \\begin{bmatrix} 1 & 0 \\\\ 0 & 3^n \\end{bmatrix} \\begin{bmatrix} 1 & -1 \\\\ 1 & 1 \\end{bmatrix} $\n",
    "\n",
    "$ = \\frac{1}{2} \\begin{bmatrix} 1 & 1 \\\\ -1 & 1 \\end{bmatrix} \\begin{bmatrix} 1 & -1 \\\\ 3^n & 3^n \\end{bmatrix} $\n",
    "\n",
    "$ = \\frac{1}{2} \\begin{bmatrix} 1 + 3^n & 1 + 3^n \\\\ -1 + 3^n & 1 + 3^n \\end{bmatrix} $\n",
    "\n",
    "Thus, the general formula for $A^n$ is:\n",
    "\n",
    "$ A^n = \\frac{1}{2} \\begin{bmatrix} 1 + 3^n & 1 + 3^n \\\\ -1 + 3^n & 1 + 3^n \\end{bmatrix} $"
   ]
  },
  {
   "cell_type": "code",
   "execution_count": null,
   "id": "11df2ff1",
   "metadata": {},
   "outputs": [],
   "source": []
  }
 ],
 "metadata": {
  "kernelspec": {
   "display_name": "SageMath 9.5",
   "language": "sage",
   "name": "sagemath"
  },
  "language_info": {
   "codemirror_mode": {
    "name": "ipython",
    "version": 3
   },
   "file_extension": ".py",
   "mimetype": "text/x-python",
   "name": "python",
   "nbconvert_exporter": "python",
   "pygments_lexer": "ipython3",
   "version": "3.10.12"
  }
 },
 "nbformat": 4,
 "nbformat_minor": 5
}
